# Bijection_Method
## Let Equation be : 
  f(x) = x*x*x - x - 4
  
## Output : 
<pre>
    a = 0  b = 2
1 : c=(0+2)/2  = 1
    f(c) = -4 < 0  , a  = c
2 : c=(1+2)/2  = 1.5
    f(c) = -2.125 < 0  , a  = c
3 : c=(1.5+2)/2  = 1.75
    f(c) = -0.390625 < 0  , a  = c
4 : c=(1.75+2)/2  = 1.875
    f(c) = 0.716797 > 0  , b  = c
5 : c=(1.75+1.875)/2  = 1.8125
    f(c) = 0.141846 > 0  , b  = c
6 : c=(1.75+1.8125)/2  = 1.78125
    f(c) = -0.129608 < 0  , a  = c
7 : c=(1.78125+1.8125)/2  = 1.79688
    f(c) = 0.0048027 > 0  , b  = c
8 : c=(1.78125+1.79688)/2  = 1.78906
    f(c) = -0.0627303 < 0  , a  = c
9 : c=(1.78906+1.79688)/2  = 1.79297
    f(c) = -0.0290459 < 0  , a  = c
10 : c=(1.79297+1.79688)/2  = 1.79492
    f(c) = -0.0121421 < 0  , a  = c
11 : c=(1.79492+1.79688)/2  = 1.7959
    f(c) = -0.00367485 < 0  , a  = c
12 : c=(1.7959+1.79688)/2  = 1.79639
    f(c) = 0.000562642 > 0  , b  = c
13 : c=(1.7959+1.79639)/2  = 1.79614
    f(c) = -0.00155643 < 0  , a  = c
14 : c=(1.79614+1.79639)/2  = 1.79626
    f(c) = -0.000496972 < 0  , a  = c
15 : c=(1.79626+1.79639)/2  = 1.79633
    f(c) = 3.28146e-005 > 0  , b  = c
16 : c=(1.79626+1.79633)/2  = 1.7963
    f(c) = -0.000232084 < 0  , a  = c
17 : c=(1.7963+1.79633)/2  = 1.79631
    f(c) = -9.96359e-005 < 0  , a  = c
18 : c=(1.79631+1.79633)/2  = 1.79632
    f(c) = -3.3411e-005 < 0  , a  = c
19 : c=(1.79632+1.79633)/2  = 1.79632
    f(c) = -2.98281e-007 < 0  , a  = c
20 : c=(1.79632+1.79633)/2  = 1.79632
    f(c) = 1.62581e-005 > 0  , b  = c
21 : c=(1.79632+1.79632)/2  = 1.79632
    f(c) = 7.97992e-006 > 0  , b  = c
22 : c=(1.79632+1.79632)/2  = 1.79632
    f(c) = 3.84082e-006 > 0  , b  = c
23 : c=(1.79632+1.79632)/2  = 1.79632
    f(c) = 1.77127e-006 > 0  , b  = c
24 : c=(1.79632+1.79632)/2  = 1.79632
    f(c) = 7.36493e-007 > 0  , b  = c
25 : c=(1.79632+1.79632)/2  = 1.79632
    f(c) = 2.19106e-007 > 0  , b  = c
26 : c=(1.79632+1.79632)/2  = 1.79632
    f(c) = -3.95878e-008 < 0  , a  = c
27 : c=(1.79632+1.79632)/2  = 1.79632
    f(c) = 8.9759e-008 > 0  , b  = c
28 : c=(1.79632+1.79632)/2  = 1.79632
    f(c) = 2.50856e-008 > 0  , b  = c
29 : c=(1.79632+1.79632)/2  = 1.79632
    f(c) = -7.25105e-009 < 0  , a  = c
30 : c=(1.79632+1.79632)/2  = 1.79632
    f(c) = 8.9173e-009 > 0  , b  = c
31 : c=(1.79632+1.79632)/2  = 1.79632
    f(c) = 8.3312e-010 > 0  , b  = c
The value of root is : 1.79632
</pre>
